More sophisticated filter example

examples/filter/filterScript.sml
@@ -12,10 +12,13 @@ val _ = new_theory "filter";
 val _ = translation_extends "chorLibProg";
 
 val n2w8 = “n2w:num -> word8”;
+val w2n = “w2n:word8 -> num”;
 
 val msg1 = “MAP (^n2w8 o ORD) "This message should be filtered."” |> EVAL |> concl |> rhs;
 val msg2 = “MAP (^n2w8 o ORD) "A message such as this should be forwarded. It is absurdly long, so hopefully it will be split into distinct messages that will all be forwarded. Indeed, that would be great, wouldn't it? Hopefully, that will be exactly the behaviour you observe when you run this example."” |> EVAL |> concl |> rhs;
 val msg3 = “MAP (^n2w8 o ORD) "Drop this message."” |> EVAL |> concl |> rhs;
+val msg4 = “MAP (^n2w8 o ORD) "A message such as this should be forwarded."” |> EVAL |> concl |> rhs;
+val msg5 = “MAP (^n2w8 o ORD) "Another message that should be forwarded."” |> EVAL |> concl |> rhs;
 
 Definition test_def :
   test args =
@@ -24,51 +27,66 @@ Definition test_def :
         else
           [0w])
 End
-
-Definition Kmsg1_def :
-  Kmsg1 args = ^msg1
+    
+Definition next_msg_def :
+  next_msg args =
+       case args of
+       | (f::r)::r' => [f+1w]
+       | _ => [0w:word8]
 End
 
-Definition Kmsg2_def :
-  Kmsg2 args = ^msg2
-End
-
-Definition Kmsg3_def :
-  Kmsg3 args = ^msg3
+Definition msg_def :
+  msg args =
+    case args of
+       | (f::r)::r' =>
+           (if f = 0w:word8 then
+             ^msg1
+           else if f=1w then ^msg2
+           else if f=2w then ^msg3
+           else if f=3w then ^msg4
+           else if f=4w then ^msg5
+           else
+             MAP (λx. ^n2w8(ORD x)) (explode (mlint$toString(&(^w2n f)))))
+       | _ => []
 End
 
 val _ = ml_prog_update (open_module "filter");
 
-val _ = next_ml_names := ["K0","K1","test","Kmsg1","Kmsg2","Kmsg3"];
-
-Theorem test_v_thm = translate test_def;
+val _ = next_ml_names := ["K0","K1","test","next_msg","msg"];
 
 Theorem K0_v_thm = translate endpoint_to_choiceTheory.K0_def;
 Theorem K1_v_thm = translate endpoint_to_choiceTheory.K1_def;
-Theorem Kmsg1_v_thm = translate Kmsg1_def;
-Theorem Kmsg2_v_thm = translate Kmsg2_def;
-Theorem Kmsg3_v_thm = translate Kmsg3_def;
+
+Theorem test_v_thm = translate test_def;
+
+Theorem next_msg_v_thm = translate next_msg_def;
+
+Theorem msg_v_thm = translate msg_def;
 
 val _ = ml_prog_update (close_module NONE);
 
 Definition filter_def:
-  filter test =
-  FOLDR (λe c.
-         Let "v" "producer" e []
-         (Com "producer" "v" "filter" "v"
-          (Let "test" "filter" test ["v"]
-           (IfThen "test" "filter"
-            (Sel "filter" T "consumer"
-             (Com "filter" "v" "consumer" "v" c)
+  (filter:chor) =
+  Let "count" "producer" K0 []
+    (Fix "X"
+       (Let "msg" "producer" msg ["count"]
+          (Let "count" "producer" next_msg ["count"]
+            (Com "producer" "msg" "filter" "msg"
+              (Let "test" "filter" test ["msg"]
+                (IfThen "test" "filter"
+                   (Sel "filter" T "consumer"
+                      (Com "filter" "msg" "consumer" "msg"
+                        (Call "X")))
+                   (Sel "filter" F "consumer"
+                        (Call "X"))
+                )
+              )
             )
-            (Sel "filter" F "consumer" c)
-           )
           )
-         )
-        )
-        chorLang$Nil
+       )
+    )
 End
 
-val thm = project_to_camkes "filter_camkes" "filter" “filter test [Kmsg1;Kmsg2;Kmsg3]”;
+val thm = project_to_camkes "filter_camkes" "filter" “filter”;
 
 val _ = export_theory();
